Limit lines to 100 characters

ulib/FStar.WellFoundedRelation.fst
@@ -24,29 +24,41 @@ open FStar.Universe
 module WF = FStar.WellFounded
 module WFU = FStar.WellFounded.Util
 
-let rec default_decreaser (#a: Type u#a) (x: a) : Tot (acc_classical (default_relation #a) x) (decreases x) =
+let rec default_decreaser (#a: Type u#a) (x: a)
+  : Tot (acc_classical (default_relation #a) x) (decreases x) =
   let smaller (y: a{default_relation y x}) : acc_classical (default_relation #a) y =
-    default_decreaser y in
+    default_decreaser y
+  in
   AccClassicalIntro smaller
 
 let default_wfr (a: Type u#a) : (wfr: wfr_t a{wfr.relation == default_relation}) =
-  let proof (x1: a) (x2: a) : Lemma (requires default_relation x1 x2) (ensures default_decreaser x1 << default_decreaser x2) =
-    assert ((default_decreaser x2).access_smaller x1 == default_decreaser x1) in
+  let proof (x1: a) (x2: a)
+    : Lemma (requires default_relation x1 x2)
+            (ensures default_decreaser x1 << default_decreaser x2) =
+    assert ((default_decreaser x2).access_smaller x1 == default_decreaser x1)
+  in
   { relation = default_relation; decreaser = default_decreaser; proof = proof; }
 
-let rec empty_decreaser (#a: Type u#a) (x: a) : Tot (acc_classical (empty_relation #a) x) (decreases x) =
+let rec empty_decreaser (#a: Type u#a) (x: a)
+  : Tot (acc_classical (empty_relation #a) x) (decreases x) =
   let smaller (y: a{empty_relation y x}) : acc_classical (empty_relation #a) y =
-    empty_decreaser y in
+    empty_decreaser y
+  in
   AccClassicalIntro smaller
 
 let empty_wfr (a: Type u#a) : (wfr: wfr_t a{wfr.relation == empty_relation}) =
-  let proof (x1: a) (x2: a) : Lemma (requires empty_relation x1 x2) (ensures empty_decreaser x1 << empty_decreaser x2) =
-    assert ((empty_decreaser x2).access_smaller x1 == empty_decreaser x1) in
+  let proof (x1: a) (x2: a)
+    : Lemma (requires empty_relation x1 x2) (ensures empty_decreaser x1 << empty_decreaser x2) =
+    assert ((empty_decreaser x2).access_smaller x1 == empty_decreaser x1)
+  in
   { relation = empty_relation; decreaser = empty_decreaser; proof = proof; }
 
-let rec acc_decreaser (#a: Type u#a) (r: a -> a -> Type0)
-                      (f: FStar.WellFounded.well_founded r{forall x1 x2 (p: r x1 x2). (f x2).access_smaller x1 p == f x1})
-                      (x: a) : Tot (acc_classical (acc_relation r) x) (decreases (f x)) =
+let rec acc_decreaser
+  (#a: Type u#a)
+  (r: a -> a -> Type0)
+  (f: FStar.WellFounded.well_founded r{forall x1 x2 (p: r x1 x2). (f x2).access_smaller x1 p == f x1})
+  (x: a)
+  : Tot (acc_classical (acc_relation r) x) (decreases (f x)) =
   let smaller (y: a{(acc_relation r) y x}) : (acc_classical (acc_relation r) y) = (
     eliminate exists (p: r y x). True
     returns   f y << f x
@@ -55,11 +67,7 @@ let rec acc_decreaser (#a: Type u#a) (r: a -> a -> Type0)
   ) in
   AccClassicalIntro smaller
 
-let rec eta_expand_well_founded
-                 (#a:Type)
-                 (r:WF.binrel a)
-                 (wf_r:WF.well_founded r)
-                 (x: a)
+let rec eta_expand_well_founded (#a: Type) (r: WF.binrel a) (wf_r: WF.well_founded r) (x: a)
   : Tot (WF.acc r x)
         (decreases {:well-founded (WFU.lift_binrel_as_well_founded_relation wf_r) (| a, x |)})
   = WF.AccIntro (let g_smaller (y: a) (u: r y x) : WF.acc r y =
@@ -67,49 +75,62 @@ let rec eta_expand_well_founded
                      eta_expand_well_founded r wf_r y
                  in g_smaller)
 
-let acc_to_wfr (#a: Type u#a)
-               (r: WF.binrel u#a u#0 a)
-               (f: FStar.WellFounded.well_founded r)
-  : (wfr: wfr_t a{wfr.relation == acc_relation r})
-  = let f = eta_expand_well_founded r f in
-    let proof (x1: a) (x2: a)
-      : Lemma (requires acc_relation r x1 x2)
-              (ensures acc_decreaser r f x1 << acc_decreaser r f x2)
-      = assert ((acc_decreaser r f x2).access_smaller x1 == acc_decreaser r f x1)
-    in
-    { relation = acc_relation r; decreaser = acc_decreaser r f; proof = proof; }
+let acc_to_wfr (#a: Type u#a) (r: WF.binrel u#a u#0 a) (f: FStar.WellFounded.well_founded r)
+  : (wfr: wfr_t a{wfr.relation == acc_relation r}) =
+  let f = eta_expand_well_founded r f in
+  let proof (x1: a) (x2: a)
+    : Lemma (requires acc_relation r x1 x2)
+            (ensures acc_decreaser r f x1 << acc_decreaser r f x2) =
+    assert ((acc_decreaser r f x2).access_smaller x1 == acc_decreaser r f x1)
+  in
+  { relation = acc_relation r; decreaser = acc_decreaser r f; proof = proof; }
 
-
-let rec subrelation_decreaser (#a: Type u#a) (r: a -> a -> Type0) (wfr: wfr_t a{forall x1 x2. r x1 x2 ==> wfr.relation x1 x2}) (x: a)
+let rec subrelation_decreaser (#a: Type u#a) (r: a -> a -> Type0)
+                              (wfr: wfr_t a{forall x1 x2. r x1 x2 ==> wfr.relation x1 x2}) (x: a)
   : Tot (acc_classical r x) (decreases wfr.decreaser x) =
   let smaller (y: a{r y x}) : (acc_classical r y) =
-    subrelation_decreaser r wfr y in
+    subrelation_decreaser r wfr y
+  in
   AccClassicalIntro smaller
 
-let subrelation_to_wfr (#a: Type u#a) (r: a -> a -> Type0) (wfr: wfr_t a{forall x1 x2. r x1 x2 ==> wfr.relation x1 x2})
+let subrelation_to_wfr (#a: Type u#a) (r: a -> a -> Type0)
+                       (wfr: wfr_t a{forall x1 x2. r x1 x2 ==> wfr.relation x1 x2})
   : (wfr': wfr_t a{wfr'.relation == r}) =
-  let proof (x1: a) (x2: a) : Lemma (requires r x1 x2) (ensures subrelation_decreaser r wfr x1 << subrelation_decreaser r wfr x2) =
-    assert ((subrelation_decreaser r wfr x2).access_smaller x1 == subrelation_decreaser r wfr x1) in
+  let proof (x1: a) (x2: a)
+     : Lemma (requires r x1 x2)
+             (ensures subrelation_decreaser r wfr x1 << subrelation_decreaser r wfr x2) =
+    assert ((subrelation_decreaser r wfr x2).access_smaller x1 == subrelation_decreaser r wfr x1)
+  in
   { relation = r; decreaser = subrelation_decreaser r wfr; proof = proof; }
 
-let rec inverse_image_decreaser  (#a: Type u#a) (#b: Type u#b) (r: a -> a -> Type0) (f: a -> b)
-                                 (wfr: wfr_t b{forall x1 x2. r x1 x2 ==> wfr.relation (f x1) (f x2)}) (x: a)
+let rec inverse_image_decreaser (#a: Type u#a) (#b: Type u#b) (r: a -> a -> Type0) (f: a -> b)
+                                (wfr: wfr_t b{forall x1 x2. r x1 x2 ==> wfr.relation (f x1) (f x2)})
+                                (x: a)
   : Tot (acc_classical r x) (decreases wfr.decreaser (f x)) =
   let smaller (y: a{r y x}) : (acc_classical r y) =
-    inverse_image_decreaser r f wfr y in
+    inverse_image_decreaser r f wfr y
+  in
   AccClassicalIntro smaller
 
 let inverse_image_to_wfr (#a: Type u#a) (#b: Type u#b) (r: a -> a -> Type0) (f: a -> b)
                          (wfr: wfr_t b{forall x1 x2. r x1 x2 ==> wfr.relation (f x1) (f x2)})
   : (wfr': wfr_t a{wfr'.relation == r}) =
-  let proof (x1: a) (x2: a) : Lemma (requires r x1 x2) (ensures inverse_image_decreaser r f wfr x1 << inverse_image_decreaser r f wfr x2) =
-    assert ((inverse_image_decreaser r f wfr x2).access_smaller x1 == inverse_image_decreaser r f wfr x1) in
+  let proof (x1: a) (x2: a)
+    : Lemma (requires r x1 x2)
+            (ensures inverse_image_decreaser r f wfr x1 << inverse_image_decreaser r f wfr x2) =
+    assert ((inverse_image_decreaser r f wfr x2).access_smaller x1 ==
+            inverse_image_decreaser r f wfr x1)
+  in
   { relation = r; decreaser = inverse_image_decreaser r f wfr; proof = proof; }
 
-let rec lex_nondep_decreaser (#a: Type u#a) (#b: Type u#b) (wfr_a: wfr_t a) (wfr_b: wfr_t b) (x: a * b)
-  : Tot (acc_classical (lex_nondep_relation wfr_a wfr_b) x) (decreases %[wfr_a.decreaser (fst x); wfr_b.decreaser (snd x)]) =
-  let smaller (y: a * b{lex_nondep_relation wfr_a wfr_b y x}) : (acc_classical (lex_nondep_relation wfr_a wfr_b) y) =
-    lex_nondep_decreaser wfr_a wfr_b y in
+let rec lex_nondep_decreaser (#a: Type u#a) (#b: Type u#b) (wfr_a: wfr_t a) (wfr_b: wfr_t b)
+                             (x: a * b)
+  : Tot (acc_classical (lex_nondep_relation wfr_a wfr_b) x)
+    (decreases %[wfr_a.decreaser (fst x); wfr_b.decreaser (snd x)]) =
+  let smaller (y: a * b{lex_nondep_relation wfr_a wfr_b y x})
+    : (acc_classical (lex_nondep_relation wfr_a wfr_b) y) =
+    lex_nondep_decreaser wfr_a wfr_b y
+  in
   AccClassicalIntro smaller
 
 let lex_nondep_wfr (#a: Type u#a) (#b: Type u#b) (wfr_a: wfr_t a) (wfr_b: wfr_t b)
@@ -117,55 +138,75 @@ let lex_nondep_wfr (#a: Type u#a) (#b: Type u#b) (wfr_a: wfr_t a) (wfr_b: wfr_t 
   let proof (x1: a * b) (x2: a * b)
     : Lemma (requires lex_nondep_relation wfr_a wfr_b x1 x2)
             (ensures  lex_nondep_decreaser wfr_a wfr_b x1 << lex_nondep_decreaser wfr_a wfr_b x2) =
-    assert ((lex_nondep_decreaser wfr_a wfr_b x2).access_smaller x1 == lex_nondep_decreaser wfr_a wfr_b x1) in
-  { relation = lex_nondep_relation wfr_a wfr_b; decreaser = lex_nondep_decreaser wfr_a wfr_b; proof = proof; }
+    assert ((lex_nondep_decreaser wfr_a wfr_b x2).access_smaller x1 ==
+            lex_nondep_decreaser wfr_a wfr_b x1)
+  in
+  { relation = lex_nondep_relation wfr_a wfr_b;
+    decreaser = lex_nondep_decreaser wfr_a wfr_b;
+    proof = proof; }
 
-let rec lex_dep_decreaser (#a: Type u#a) (#b: a -> Type u#b) (wfr_a: wfr_t a) (a_to_wfr_b: (x: a -> wfr_t (b x))) (x: (v: a & b v))
+let rec lex_dep_decreaser (#a: Type u#a) (#b: a -> Type u#b) (wfr_a: wfr_t a)
+                          (a_to_wfr_b: (x: a -> wfr_t (b x))) (x: (v: a & b v))
   : Tot (acc_classical (lex_dep_relation wfr_a a_to_wfr_b) x)
         (decreases %[wfr_a.decreaser (dfst x); (a_to_wfr_b (dfst x)).decreaser (dsnd x)]) =
-  let smaller (y: (v: a & b v){lex_dep_relation wfr_a a_to_wfr_b y x}) : (acc_classical (lex_dep_relation wfr_a a_to_wfr_b) y) =
-    lex_dep_decreaser wfr_a a_to_wfr_b y in
+  let smaller (y: (v: a & b v){lex_dep_relation wfr_a a_to_wfr_b y x})
+    : (acc_classical (lex_dep_relation wfr_a a_to_wfr_b) y) =
+    lex_dep_decreaser wfr_a a_to_wfr_b y
+  in
   AccClassicalIntro smaller
 
-let lex_dep_wfr (#a: Type u#a) (#b: a -> Type u#b) (wfr_a: wfr_t a) (a_to_wfr_b: (x: a -> wfr_t (b x)))
+let lex_dep_wfr (#a: Type u#a) (#b: a -> Type u#b) (wfr_a: wfr_t a)
+                (a_to_wfr_b: (x: a -> wfr_t (b x)))
   : wfr: wfr_t (x: a & b x){wfr.relation == lex_dep_relation wfr_a a_to_wfr_b} =
   let proof (x1: (v: a & b v)) (x2: (v: a) & b v)
     : Lemma (requires lex_dep_relation wfr_a a_to_wfr_b x1 x2)
-            (ensures  lex_dep_decreaser wfr_a a_to_wfr_b x1 << lex_dep_decreaser wfr_a a_to_wfr_b x2) =
-    assert ((lex_dep_decreaser wfr_a a_to_wfr_b x2).access_smaller x1 == lex_dep_decreaser wfr_a a_to_wfr_b x1) in
-  { relation = lex_dep_relation wfr_a a_to_wfr_b; decreaser = lex_dep_decreaser wfr_a a_to_wfr_b; proof = proof; }
+            (ensures  lex_dep_decreaser wfr_a a_to_wfr_b x1 <<
+                      lex_dep_decreaser wfr_a a_to_wfr_b x2) =
+    assert ((lex_dep_decreaser wfr_a a_to_wfr_b x2).access_smaller x1 ==
+            lex_dep_decreaser wfr_a a_to_wfr_b x1)
+  in
+  { relation = lex_dep_relation wfr_a a_to_wfr_b;
+    decreaser = lex_dep_decreaser wfr_a a_to_wfr_b;
+    proof = proof; }
 
 let bool_wfr: (wfr: wfr_t bool{wfr.relation == bool_relation}) =
   inverse_image_to_wfr #bool #nat bool_relation (fun b -> if b then 1 else 0) (default_wfr nat)
 
-let option_wfr (#a: Type u#a) (wfr: wfr_t a) : wfr': wfr_t (option a){wfr'.relation == option_relation wfr} =
+let option_wfr (#a: Type u#a) (wfr: wfr_t a)
+  : wfr': wfr_t (option a){wfr'.relation == option_relation wfr} =
   // We'll need the unit type raised to universe u#a
 
   let unit_a: Type u#a = raise_t unit in
 
-  // Step 1:  Create a function f mapping an `option a` to a `(b: bool & (if b then a else unit_a))`.
-  //          It should map `Some x` to `(| true, x |)` and `None` to `(| false, () |)`.
+  // Step 1: Create a function f mapping an `option a` to a
+  //          `(b: bool & (if b then a else unit_a))`.  It should map
+  //          `Some x` to `(| true, x |)` and `None` to `(| false, () |)`.
 
   let f: option a -> (b: bool & (if b then a else unit_a)) =
-    fun opt -> (match opt with | Some x -> (| true, x |) | None -> (| false, raise_val () |) ) in
+    fun opt -> (match opt with | Some x -> (| true, x |) | None -> (| false, raise_val () |) )
+  in
 
   // Step 2:  Create a wfr for (b: bool & (if b then a else unit_a)) using lex_dep_wfr.
   //          The precedence for the bool field should be bool_wfr (i.e., false precedes true).
-  //          The precedence for the (if b then a else unit_a) field should be either wfr or empty_wfr,
-  //          depending on whether b is true or false.
+  //          The precedence for the (if b then a else unit_a) field should be either wfr or
+  //          empty_wfr, depending on whether b is true or false.
 
-  let bool_to_wfr_a (b: bool) : wfr_t (if b then a else unit_a) = if b then wfr else empty_wfr unit_a in
-  let wfr_bool_a: wfr_t (b: bool & (if b then a else unit_a)) = lex_dep_wfr bool_wfr bool_to_wfr_a in
+  let bool_to_wfr_a (b: bool) : wfr_t (if b then a else unit_a) =
+    if b then wfr else empty_wfr unit_a
+  in
+  let wfr_bool_a: wfr_t (b: bool & (if b then a else unit_a)) =
+    lex_dep_wfr bool_wfr bool_to_wfr_a
+  in
 
-  assert (forall (bx1: (b: bool & (if b then a else unit_a))) (bx2: (b: bool & (if b then a else unit_a))).
+  assert (forall (bx1: (b: bool & (if b then a else unit_a)))
+            (bx2: (b: bool & (if b then a else unit_a))).
             wfr_bool_a.relation bx1 bx2 <==>
                (let (| b1, x1 |), (| b2, x2 |) = bx1, bx2 in
                 (not b1 && b2) \/ (b1 && b2 /\ wfr.relation x1 x2)));
 
-  // Step 3:  Create the final wfr using inverse_image_to_wfr, using `f` as the mapping function from
-  //          `option a` to `(b: bool & (if b then a else unit_a))` and `wfr_bool_a` as the wfr_t
-  //          for `(b: bool & (if b then a else unit_a))`.
+  // Step 3:  Create the final wfr using inverse_image_to_wfr, using `f` as the mapping
+  //          function from `option a` to `(b: bool & (if b then a else unit_a))` and
+  //          `wfr_bool_a` as the wfr_t for `(b: bool & (if b then a else unit_a))`.
 
   assert (forall opt1 opt2. (option_relation wfr) opt1 opt2 ==> wfr_bool_a.relation (f opt1) (f opt2));
   inverse_image_to_wfr (option_relation wfr) f wfr_bool_a
-
